Borda refined and verified

theories/Compositional_Structures/Basic_Modules/Component_Types/Evaluation_Function_Ref.thy
@@ -23,7 +23,7 @@ subsection \<open>Definition\<close>
 
 type_synonym 'a Evaluation_Function_Ref = "'a  \<Rightarrow> 'a set \<Rightarrow> 'a Profile_List \<Rightarrow> nat nres"
 
-abbreviation "evalf_rel \<equiv> Id \<rightarrow> \<langle>Id\<rangle>set_rel \<rightarrow> profile_rel \<rightarrow> \<langle>nat_rel\<rangle>nres_rel"
+abbreviation "evalf_rel \<equiv> Id  \<rightarrow> profile_rel \<rightarrow> \<langle>nat_rel\<rangle>nres_rel"
 
 abbreviation "evalf_profA_rel A \<equiv> Id \<rightarrow> profile_on_A_rel A \<rightarrow> \<langle>nat_rel\<rangle>nres_rel"
 
@@ -34,9 +34,9 @@ lemma evalfeq:
   fixes pl :: "'a Profile_List"
   assumes 
      pref: "(pl, pr) \<in> profile_rel" and
-     evalref: "((\<lambda> a A pl . refn a A pl), (\<lambda> a A pr. RETURN (efn a A pr))) \<in> evalf_rel"
+     evalref: "((\<lambda> a pl . refn a A pl), (\<lambda> a pr. RETURN (efn a A pr))) \<in> evalf_rel"
   shows "refn a A pl \<le> RETURN (efn a A pr)"
-  using assms(1) assms(2)[THEN fun_relD, THEN fun_relD,THEN fun_relD, THEN nres_relD]
+  using pref evalref[THEN fun_relD,THEN fun_relD, THEN nres_relD]
   by auto
   
   subsection \<open>Refined Condorcet Property\<close>
@@ -55,75 +55,6 @@ definition condorcet_rating_mon_aux :: "'a Evaluation_Function_Ref
       sw <- f w A p;
       sl <- f x A p;
       RETURN (b \<and> (sl < sw))}) (True)"
-
-definition condorcet_rating_mon :: "'a Evaluation_Function_Ref \<Rightarrow> bool" where
-  "condorcet_rating_mon f \<equiv> 
-       \<forall> A p w . 
-      (condorcet_winner_l A p w \<longrightarrow>  
-    (\<forall> l \<in> A . l \<noteq> w \<longrightarrow> do { sw <- f w A p;
-      sl <- f l A p; RETURN (sl < sw)} \<le> RETURN (True)))"
-
-definition refines_cond_rating :: "'a Evaluation_Function_Ref \<Rightarrow> bool" where
-  "refines_cond_rating eref \<equiv> \<exists> efn:: 'a Evaluation_Function . 
-      (eref, (\<lambda> a Alts pro. RETURN (efn a Alts pro))) \<in> evalf_rel
-      \<and> condorcet_rating efn
-    "
-  
-
-lemma condorcet_rating_ref_refine:
-  fixes eref :: "'a Evaluation_Function_Ref"
-  and e :: "'a Evaluation_Function"
-  assumes evalfref: "(eref, (\<lambda> a Alts pro. RETURN (efn a Alts pro))) \<in> evalf_rel"
-  shows "condorcet_rating efn \<longleftrightarrow> condorcet_rating_mon eref"
-proof (unfold condorcet_rating_mon_def condorcet_rating_def condorcet_rating_mon_aux_def, safe)
-  fix A :: "'a set"
-  fix pl:: "'a Profile_List"
-  fix w :: 'a
-  fix l :: 'a
-  assume lA: "l \<in> A"
-  assume wnl: "l \<noteq> w"
-  assume pre: "\<forall>A p w. condorcet_winner A p w \<longrightarrow> (\<forall>l\<in>A. l \<noteq> w \<longrightarrow> efn l A p < efn w A p)"
-  assume winner: "condorcet_winner_l A pl w"
-  from winner have fina: "finite A" by simp
-  from winner have "RETURN (condorcet_winner_l A pl w) = RETURN True" by simp
-    from winner have profl: "profile_l A pl" by simp
-  from this obtain pr where "pr = map pl_\<alpha> pl"
-    by blast
- from this profl have profilerel: "(pl, pr) \<in> profile_rel" unfolding profile_l_def
-    by (metis in_set_conv_nth map_in_list_rel_conv)
-  note efeq = evalfref[THEN fun_relD, THEN fun_relD, THEN fun_relD, THEN nres_relD,
-      where x2 = A and x'2 = A and x1 = "pl" and x'1 = pr]
-  note cc = condorcet_winner_l_correct[THEN fun_relD, THEN fun_relD, THEN fun_relD,
-      where x2 = A and x'2 = A and x1 = pl and x'1 = pr and x = w and x' = w]
-  from profilerel winner cc have cwpr: "condorcet_winner A pr w"
-    by (metis pair_in_Id_conv set_relI)
-  from this lA wnl pre have concond: "efn l A pr < efn w A pr" by simp
-  from profilerel efeq have eqsl: "eref l A pl \<le> RETURN (efn l A pr)"
-    by simp 
-  from profilerel efeq have eqsw: "eref w A pl \<le> RETURN (efn w A pr)"
-    by simp 
-  from concond lA wnl profilerel eqsl eqsw 
-  show  "eref w A pl \<bind> (\<lambda>sw. eref l A pl \<bind> (\<lambda>sl. RETURN (sl < sw))) \<le> RETURN True"
-    using RETURN_SPEC_conv SPEC_cons_rule plain_RETURN specify_left
-    by (smt (verit, best))
-next 
-  fix A :: "'a set"
-  fix pr:: "'a Profile"
-  fix w :: 'a
-  fix l :: 'a
-  assume lA: "l \<in> A"
-  assume wnl: "l \<noteq> w"
-  assume winner: "condorcet_winner A pr w"
-  assume crref: " \<forall>A p w.
-          condorcet_winner_l A p w \<longrightarrow>
-          (\<forall>l\<in>A. l \<noteq> w \<longrightarrow> eref w A p \<bind> (\<lambda>sw. eref l A p \<bind> (\<lambda>sl. RETURN (sl < sw))) \<le> RETURN True)"
-  from winner have "finite_profile A pr" by simp
-  note cc = condorcet_winner_l_correct[THEN fun_relD, THEN fun_relD, THEN fun_relD,
-      where x2 = A and x'2 = A  and x'1 = pr and x = w and x' = w]
-  from lA wnl winner crref cc show "efn l A pr < efn w A pr"
-    oops
-
-
          
 subsection \<open>Theorems\<close>
 
@@ -133,18 +64,19 @@ text \<open>
 \<close>
 
 theorem cond_winner_imp_max_eval_val_ref:
+  fixes A :: "'a set"
   fixes eref :: "'a Evaluation_Function_Ref"
   and efn :: "'a Evaluation_Function"
   fixes pl :: "'a Profile_List" and pr :: "'a Profile"
   assumes profrel : "(pl, pr) \<in> profile_rel"
-  assumes evalfref: "(eref, (\<lambda> a Alts pro. RETURN (efn a Alts pro))) \<in> evalf_rel"
+  assumes evalfref: "((\<lambda> a pro. eref a A pro), (\<lambda> a  pro. RETURN (efn a A pro))) \<in> evalf_rel"
   assumes
     rating: "condorcet_rating efn" and
     fina: "finite A" and profl: "profile_l A pl" and
     winnerl: "condorcet_winner_l A pl w"
   shows "eref w A pl \<le> RETURN (Max {efn a A pr | a. a \<in> A})"
 proof -
-  note efeq = evalfref[THEN fun_relD, THEN fun_relD, THEN fun_relD, THEN nres_relD]
+  note efeq = evalfref[THEN fun_relD, THEN fun_relD, THEN nres_relD]
   from this have efref: "eref w A pl \<le> RETURN (efn w A pr)"
     using profrel refine_IdD
     by simp
@@ -155,8 +87,7 @@ proof -
   profrel
   have winner: "condorcet_winner A pr w"
     by (metis pair_in_Id_conv set_rel_id)
-  note efi = efeq[where x3 = w and x'3 = w and x2 = A and x'2 = A
-      and x1 = pl and x'1 = pr]
+  note efi = efeq[where x2 = w and x'2 = w and x1 = pl and x'1 = pr]
   from rating f_prof winner
   have "efn w A pr = Max {efn a A pr |a. a \<in> A}" using cond_winner_imp_max_eval_val
     by (metis (mono_tags, lifting))
@@ -176,7 +107,7 @@ theorem non_cond_winner_not_max_eval_ref:
   and efn :: "'a Evaluation_Function"
   fixes pl :: "'a Profile_List" and pr :: "'a Profile"
   assumes profrel : "(pl, pr) \<in> profile_rel"
-  assumes evalfref: "(eref, (\<lambda> a Alts pro. RETURN (efn a Alts pro))) \<in> evalf_rel"
+  assumes evalfref: "((\<lambda> a pro. eref a A pro), (\<lambda> a pro. RETURN (efn a A pro))) \<in> evalf_rel"
   assumes
     rating: "condorcet_rating efn" and
     fina: "finite A" and profl: "profile_l A pl" and
@@ -185,7 +116,7 @@ theorem non_cond_winner_not_max_eval_ref:
     loser: "w \<noteq> l"
   shows "do {sl <- eref l A pl; RETURN (sl < Max {efn a A pr | a. a \<in> A})} \<le> RETURN True"  
 proof -
-   note efeq = evalfref[THEN fun_relD, THEN fun_relD, THEN fun_relD, THEN nres_relD]
+   note efeq = evalfref[THEN fun_relD, THEN fun_relD, THEN nres_relD]
   from this have efref: "eref w A pl \<le> RETURN (efn w A pr)"
     using profrel refine_IdD
     by simp
